MatMul.Kernel: add fsti

src/examples/matmul/GPU.MatMul.Kernel.fst
@@ -1,5 +1,73 @@
 module GPU.MatMul.Kernel
 
+inline_for_extraction let hack = 1
+
 #lang-pulse
 
 open GPU
+module SZ = FStar.SizeT
+
+#set-options "--z3rlimit 20"
+
+[@@CPrologue "__global__"]
+fn kernel
+  // (rows: nat) (shared: nat { shared < pow2 16 }) (columns: nat)
+  (ga1 : gpu_array u64 (rows * shared))
+  (ga2 : gpu_array u64 (shared * columns))
+  (r : gpu_array u64 (rows * columns))
+  (#s1: erased (seq u64) {Seq.length s1 == rows * shared})
+  (#s2: erased (seq u64) {Seq.length s2 == shared * columns})
+  (nth : erased sz { SZ.v nth == SZ.v SZ.(rows *^ columns) })
+  (etid : erased tid_t { gdim_x etid == nth /\ bdim_x etid == 1sz })
+  requires gpu
+    ** thread_id etid
+    ** kpre rows shared columns ga1 ga2 r #s1 #s2 (SZ.v nth) (thread_index etid)
+  ensures  gpu
+    ** thread_id etid
+    ** kpost rows shared columns ga1 ga2 r #s1 #s2 (SZ.v nth) (thread_index etid)
+{
+  open FStar.SizeT;
+
+  let tid = block_idx_x () <: u32;
+  let tid : sz = SZ.uint32_to_sizet tid;
+
+  (* r[tid] = TODO *)
+  let trow = SZ.div tid columns;
+  let tcol = SZ.rem tid columns;
+  // assert (pure (0 <= trow /\ trow < rows /\ 0 <= tcol /\ tcol < columns));
+
+  let mut i = 0sz;
+  let mut sum = 0UL;
+
+  while (let v = !i; (v <^ shared))
+     invariant b.
+       exists* v.
+       pure (0 <= shared /\ b == (SZ.v v < shared) /\ SZ.v v <= shared /\ SZ.v v >= 0) **
+       pts_to i v **
+       gpu **
+       pts_to sum (Pure.matmul_single rows shared columns s1 s2 trow tcol (SZ.v v))
+       ** Impure.gpu_pts_to_matrix #u64 rows shared ga1 (SZ.v nth) s1
+       ** Impure.gpu_pts_to_matrix #u64 shared columns ga2 (SZ.v nth) s2
+  {
+    let v = !i;
+    let s = !sum;
+    let v1 = Impure.gpu_matrix_read #_ #rows #shared ga1 #(SZ.v nth) #s1 trow v;
+    let v2 = Impure.gpu_matrix_read #_ #shared #columns ga2 #(SZ.v nth) #s2 v tcol;
+
+    i := SZ.add v 1sz;
+    sum := U64.add_mod (U64.mul_mod v1 v2) s;
+
+    (**)Pure.matmul_single_lemma rows shared columns s1 s2 trow tcol (SZ.v (SZ.add v 1sz));
+    ()
+  };
+
+  let s = !sum;
+  gpu_array_write #u64 #(rows * columns) #((SZ.v tid)) #((SZ.v tid + 1)) r tid s;
+
+  with #v. assert (gpu_pts_to_array_slice r tid (tid + 1) v);
+  (**)Seq.lemma_eq_intro v seq![s];
+  (**)rewrite gpu_pts_to_array_slice r tid (tid + 1) v
+    as gpu_pts_to_array_slice r tid (tid + 1) seq![s];
+
+  ()
+}
