src/examples/matmul/GPU.MatMul.Kernel.fsti
@@ -1,5 +1,8 @@
 module GPU.MatMul.Kernel
 
+(* THIS IS NEEDED SO F* WILL ACTUALLY DO CROSS-MODULE INLINING. *)
+inline_for_extraction val hack : int
+
 #lang-pulse
 
 #push-options "--fuel 1 --ifuel 1"
@@ -82,49 +85,3 @@ fn kernel
   ensures  gpu
     ** thread_id etid
     ** kpost rows shared columns ga1 ga2 r #s1 #s2 (SZ.v nth) (thread_index etid)
-{
-  open FStar.SizeT;
-
-  let tid = block_idx_x () <: u32;
-  let tid : sz = SZ.uint32_to_sizet tid;
-
-  (* r[tid] = TODO *)
-  let trow = SZ.div tid columns;
-  let tcol = SZ.rem tid columns;
-  // assert (pure (0 <= trow /\ trow < rows /\ 0 <= tcol /\ tcol < columns));
-
-  let mut i = 0sz;
-  let mut sum = 0UL;
-
-  while (let v = !i; (v <^ shared))
-     invariant b.
-       exists* v.
-       pure (0 <= shared /\ b == (SZ.v v < shared) /\ SZ.v v <= shared /\ SZ.v v >= 0) **
-       pts_to i v **
-       gpu **
-       pts_to sum (Pure.matmul_single rows shared columns s1 s2 trow tcol (SZ.v v))
-       ** Impure.gpu_pts_to_matrix #u64 rows shared ga1 (SZ.v nth) s1
-       ** Impure.gpu_pts_to_matrix #u64 shared columns ga2 (SZ.v nth) s2
-  {
-    let v = !i;
-    let s = !sum;
-    let v1 = Impure.gpu_matrix_read #_ #rows #shared ga1 #(SZ.v nth) #s1 trow v;
-    let v2 = Impure.gpu_matrix_read #_ #shared #columns ga2 #(SZ.v nth) #s2 v tcol;
-
-    i := SZ.add v 1sz;
-    sum := U64.add_mod (U64.mul_mod v1 v2) s;
-
-    (**)Pure.matmul_single_lemma rows shared columns s1 s2 trow tcol (SZ.v (SZ.add v 1sz));
-    ()
-  };
-
-  let s = !sum;
-  gpu_array_write #u64 #(rows * columns) #((SZ.v tid)) #((SZ.v tid + 1)) r tid s;
-
-  with #v. assert (gpu_pts_to_array_slice r tid (tid + 1) v);
-  (**)Seq.lemma_eq_intro v seq![s];
-  (**)rewrite gpu_pts_to_array_slice r tid (tid + 1) v
-    as gpu_pts_to_array_slice r tid (tid + 1) seq![s];
-
-  ()
-}
